ocaml2zoo: Handle std/inf_array.

theories/std/inf_array.ml
@@ -1,0 +1,33 @@
+type 'a t =
+  { mutable data: 'a array;
+    default: 'a;
+    mutex: Mutex.t;
+  }
+
+let create default =
+  let data = Array.create () in
+  let mutex = Mutex.create () in
+  { data; default; mutex }
+
+let get t i =
+  Mutex.protect t.mutex (fun () ->
+    let data = t.data in
+    if i < Array.size data then (
+      Array.unsafe_get data i
+    ) else (
+      t.default
+    )
+  )
+
+let set t i v =
+  Mutex.protect t.mutex (fun () ->
+    let data = t.data in
+    let sz = Array.size data in
+    if i < sz then (
+      Array.unsafe_set data i v
+    ) else (
+      let data = Array.unsafe_grow data (1 + i) t.default in
+      t.data <- data ;
+      Array.unsafe_set data i v
+    )
+  )
