theories/std/inf_array__types.v
@@ -1,0 +1,22 @@
+From zoo Require Import
+  prelude.
+From zoo.language Require Import
+  notations.
+From zoo.std Require Import
+  array
+  mutex.
+From zoo Require Import
+  options.
+
+Notation "'data'" := (
+  in_type "t" 0
+)(in custom zoo_field
+).
+Notation "'default'" := (
+  in_type "t" 1
+)(in custom zoo_field
+).
+Notation "'mutex'" := (
+  in_type "t" 2
+)(in custom zoo_field
+).
